mark-and-sweep/spec/GC.Spec.ChunkedSweepCoalesce.Compat.fsti
@@ -1,0 +1,35 @@
+module GC.Spec.ChunkedSweepCoalesce.Compat
+
+module U64 = FStar.UInt64
+
+open GC.Spec.Base
+open GC.Spec.Heap
+
+module Header = GC.Lib.Header
+module MH = GC.Spec.MajorHeap
+module Obj = GC.Spec.Object
+module Defs = GC.Spec.ChunkedSweepCoalesce.Defs
+module SpecSweep = GC.Spec.Sweep
+
+val chunked_make_white_single_chunk_compat
+  (g: heap)
+  (obj: obj_addr{U64.v obj >= U64.v zero_addr + U64.v mword})
+  : Lemma
+      (Defs.chunked_make_white (MH.single_chunk_major_heap g) obj ==
+       MH.single_chunk_major_heap (Obj.makeWhite obj g))
+
+val chunked_make_blue_single_chunk_compat
+  (g: heap)
+  (obj: obj_addr{U64.v obj >= U64.v zero_addr + U64.v mword})
+  : Lemma
+      (Defs.chunked_make_blue (MH.single_chunk_major_heap g) obj ==
+       MH.single_chunk_major_heap (Obj.makeBlue obj g))
+
+val chunked_sweep_object_single_chunk_compat
+  (g: heap)
+  (obj: obj_addr{U64.v obj >= U64.v zero_addr + U64.v mword})
+  (fp: U64.t)
+  : Lemma
+      (Defs.chunked_sweep_object (MH.single_chunk_major_heap g) obj fp ==
+       (let (g', fp') = SpecSweep.sweep_object g obj fp in
+        (MH.single_chunk_major_heap g', fp')))
